\documentclass{article}

\usepackage[utf8]{inputenc}
\usepackage{ctex}
\usepackage{assignpkg}
\usepackage{amsmath}
\usepackage{amssymb}
\studentIds{202XX80XXXXXXXX}{}
\studentNames{XXX}{}

\assignmentNumber{3}

\date{\today}

\begin{document}

\makecover
求证：\[H(XY)=H(X)+H(Y)-I(X;Y)\]
证明：
\begin{align*}
H(XY)+I(X;Y)&=-(\sum_{i=1}^n \sum_{j=1}^m P(x_i, y_j)log_2P(x_i,y_j)+\sum_{i=1}^n \sum_{j=1}^m P(x_i,y_j)log_2\frac{P(x_i)}{P(x_i|y_j)})\\
&=-(\sum_{i=1}^n\sum_{j=1}^m P(x_i,y_j)log_2(\frac{P(x_i,y_j)P(x_i)}{P(x_i|y_j)}))\\
&=-(\sum_{i=1}^n\sum_{j=1}^mP(x_i,y_j)log_2\frac{P(y_j)P(x_i|y_j)P(x_i)}{P(x_i|y_j)})\\
&=-(\sum_{i=1}^n\sum_{j=1}^mP(x_i,y_j)log_2(P(x_i)P(y_j)))\\
&=-(\sum_{i=1}^n\sum_{j=1}^mP(x_i,y_j)log_2P(x_i) + \sum_{i=1}^n\sum_{j=1}^m P(x_i,y_j)log_2P(y_j))\\
&=-(\sum_{i=1}^n(\sum_{j=1}^m P(x_i,y_j))log_2P(x_i) + \sum_{j=1}^m(\sum_{i=1}^nP(x_i,y_j))P(y_j))\\
&=-(\sum_{i=1}^nP(x_i)log_2P(x_i) + \sum_{j=1}^mP(y_j)log_2P(y_j))\\
&=H(X)+H(Y)\\
\end{align*}
故命题得证。
\end{document}








